Add back cocpar

syntax.sig
@@ -1,6 +1,9 @@
 Tm(VarTm) : Type
 Ty(VarTy) : Type
+CTm(VarCTm) : Type
+
 Ki : Type
+CSort : Type
 
 TmAbs : (bind Tm in Tm) -> Tm
 TmApp : Tm -> Tm -> Tm
@@ -12,3 +15,11 @@ TyFun : Ty -> Ty -> Ty
 
 Star : Ki
 Arr : Ki -> Ki -> Ki
+
+CStar : CSort
+CKind : CSort
+
+CTmAbs : (bind CTm in CTm) -> CTm
+CTmApp : CTm -> CTm -> CTm
+CTmForall : CTm -> (bind CTm in CTm) -> CTm
+CTmSort : CSort -> CTm
